# inverse of a complex number
The inverse number if multiplied by the inverted number results in $1$
## inverse of a complex number in algebraic notation
The inverse number if multiplied by the inverted number results in $1$
$$\frac{z_1}{z_2}=z_1z_2^{-1}=(x+iy)(\frac{x}{x^2+y^2}-\frac{iy}{x^2+y^2})$$
$$

\begin{align}
z^{-1}&= \frac{1}{z} \\ 
&= \frac{1}{z}\cdot\frac{\overline{z}}{\overline{z}}\\
&= \frac{1}{z+iy}\cdot\frac{x-iy}{x-iy} \\
&=\frac{x-iy}{x^2+y^2} \\
&= \frac{x}{x^2+y^2}-\frac{iy}{x^2+y^2}
\end{align}
$$
## inverse of a complex number in polar notation
$$
z^{-1}=(re^{i\theta})^{-1}=r^{-1}(e^{i\theta})^{-1}=\frac{1}{r}e^{i(-\theta)}
$$